checkpoint thinking about txn layer specs

src/program_proof/txn/specs.v
@@ -1,30 +1,26 @@
 From RecordUpdate Require Import RecordSet.
 Import RecordSetNotations.
 
+(*
+  TODO: get txn to actually Goose
+  TODO: allow representing multiple logical disks with Txn,
+    one per logical disk from Wal.
+  TODO: how to deal with crashes?  the 3 ghost maps exposed
+    by Txn must remain latest, so what represents the old state?
+*)
+
 From Perennial.Helpers Require Import Transitions.
 From Perennial.program_proof Require Import proof_prelude.
 
-Record addr := {
-  addr_block : u64;
-  addr_offset : u64;
-}.
-
-Global Instance addr_eq_dec : EqDecision addr.
-Proof.
-  intros x y.
-  destruct x; destruct y.
-  destruct (decide (addr_block0 = addr_block1)).
-  - destruct (decide (addr_offset0 = addr_offset1)).
-    + left; congruence.
-    + right; congruence.
-  - right; congruence.
-Defined.
-
-Global Instance addr_finite : Countable addr.
-Admitted.
+From Goose.github_com.mit_pdos.goose_nfsd Require Import buf.
 
 Definition inode_bytes := Z.to_nat 128.
 Definition inode_buf := vec u8 inode_bytes.
+Definition inode_to_vals {ext: ext_op} (i:inode_buf) : list val :=
+  fmap b2val (vec_to_list i).
+
+Definition inode_bits : u64 := inode_bytes*8.
+Definition block_bits : u64 := block_bytes*8.
 
 Inductive updatable_buf (T : Type) :=
 | Stable : forall (v : T), updatable_buf T
@@ -36,15 +32,21 @@ Arguments Stable {T} v.
 Section heap.
 Context `{!heapG Σ}.
 Context `{!lockG Σ}.
-Context `{!gen_heapPreG u64 (gen_heapG u64 (updatable_buf Block) Σ) Σ}.
-Context `{!gen_heapPreG u64 (gen_heapG u64 (updatable_buf inode_buf) Σ) Σ}.
-Context `{!gen_heapPreG u64 (gen_heapG u64 (updatable_buf bool) Σ) Σ}.
 Context `{!gen_heapPreG u64 Block Σ}.
+Context `{!gen_heapPreG u64 (updatable_buf Block) Σ}.
+Context `{!gen_heapPreG u64 (updatable_buf inode_buf) Σ}.
+Context `{!gen_heapPreG u64 (updatable_buf bool) Σ}.
+Context `{!gen_heapPreG unit
+          (gmap u64 (gmap u64 (updatable_buf bool)) *
+           gmap u64 (gmap u64 (updatable_buf inode_buf)) *
+           gmap u64 (gmap u64 (updatable_buf Block)))
+         Σ}.
 
 Implicit Types s : Slice.t.
 Implicit Types (stk:stuckness) (E: coPset).
 
-Definition lockN : namespace := nroot .@ "txn".
+Definition lockN : namespace := nroot .@ "txnlock".
+Definition invN : namespace := nroot .@ "txninv".
 
 Definition txn_inodes_in_block (b : Block) (gm : gmap u64 (updatable_buf inode_buf)) : iProp Σ :=
   (
@@ -80,13 +82,173 @@ Definition txn_blocks_in_block (b : Block) (gm : gmap u64 (updatable_buf Block))
       end
   )%I.
 
-Definition is_txn (lt : loc) (walHeap : gen_heapG u64 Block Σ)
-    (gBits   : gen_heapG u64 (gen_heapG u64 (updatable_buf bool) Σ) Σ)
-    (gInodes : gen_heapG u64 (gen_heapG u64 (updatable_buf inode_buf) Σ) Σ)
-    (gBlocks : gen_heapG u64 (gen_heapG u64 (updatable_buf Block) Σ) Σ)
+Definition is_txn_always (walHeap : gen_heapG u64 Block Σ)
+    (gBits   : gmap u64 (gen_heapG u64 (updatable_buf bool) Σ))
+    (gInodes : gmap u64 (gen_heapG u64 (updatable_buf inode_buf) Σ))
+    (gBlocks : gmap u64 (gen_heapG u64 (updatable_buf Block) Σ))
+    γMaps
     : iProp Σ :=
   (
-    True
+    ∃ (mBits : gmap u64 (gmap u64 (updatable_buf bool)))
+      (mInodes : gmap u64 (gmap u64 (updatable_buf inode_buf)))
+      (mBlocks : gmap u64 (gmap u64 (updatable_buf Block))),
+      ( [∗ map] blkno ↦ gm;gh ∈ mBits;gBits, gen_heap_ctx (hG := gh) gm ) ∗
+      ( [∗ map] blkno ↦ gm;gh ∈ mInodes;gInodes, gen_heap_ctx (hG := gh) gm ) ∗
+      ( [∗ map] blkno ↦ gm;gh ∈ mBlocks;gBlocks, gen_heap_ctx (hG := gh) gm ) ∗
+      mapsto (hG := γMaps) tt (1/2) (mBits, mInodes, mBlocks) ∗
+      ( [∗ map] blkno ↦ bitmap ∈ mBits,
+          ∃ b,
+            mapsto (hG := walHeap) blkno 1 b ∗
+            txn_bits_in_block b bitmap ) ∗
+      ( [∗ map] blkno ↦ inodemap ∈ mInodes,
+          ∃ b,
+            mapsto (hG := walHeap) blkno 1 b ∗
+            txn_inodes_in_block b inodemap ) ∗
+      ( [∗ map] blkno ↦ blockmap ∈ mBlocks,
+          ∃ b,
+            mapsto (hG := walHeap) blkno 1 b ∗
+            txn_blocks_in_block b blockmap )
   )%I.
+
+Definition is_txn_locked γMaps : iProp Σ :=
+  (
+    ∃ (mBits : gmap u64 (gmap u64 (updatable_buf bool)))
+      (mInodes : gmap u64 (gmap u64 (updatable_buf inode_buf)))
+      (mBlocks : gmap u64 (gmap u64 (updatable_buf Block))),
+      mapsto (hG := γMaps) tt (1/2) (mBits, mInodes, mBlocks) ∗
+      ( [∗ map] blkno ↦ bitmap ∈ mBits,
+          [∗ map] off ↦ ub_bit ∈ bitmap, ⌜ub_bit ≠ Unstable⌝ ) ∗
+      ( [∗ map] blkno ↦ inodemap ∈ mBits,
+          [∗ map] off ↦ ub_inode ∈ inodemap, ⌜ub_inode ≠ Unstable⌝ ) ∗
+      ( [∗ map] blkno ↦ blockmap ∈ mBits,
+          [∗ map] off ↦ ub_block ∈ blockmap, ⌜ub_block ≠ Unstable⌝ )
+  )%I.
+
+Definition is_txn (l : loc)
+    (gBits   : gmap u64 (gen_heapG u64 (updatable_buf bool) Σ))
+    (gInodes : gmap u64 (gen_heapG u64 (updatable_buf inode_buf) Σ))
+    (gBlocks : gmap u64 (gen_heapG u64 (updatable_buf Block) Σ))
+    : iProp Σ :=
+  (
+    ∃ γMaps γLock (walHeap : gen_heapG u64 Block Σ),
+      (* Say something about the struct Txn stored at l,
+         get the [*wal.Walog] from l, and connect that
+         to wal_Heap. *)
+      inv invN (is_txn_always walHeap gBits gInodes gBlocks γMaps) ∗
+      is_lock lockN γLock #l (is_txn_locked γMaps)
+  )%I.
+
+Axiom txn_Load : val.
+
+Theorem wp_txn_Load_bit l gBits gInodes gBlocks (blk off : u64)
+    (hG : gen_heapG u64 (updatable_buf bool) Σ) v :
+  {{{ is_txn l gBits gInodes gBlocks ∗
+      ⌜gBits !! blk = Some hG⌝ ∗
+      mapsto (hG := hG) off 1 (Stable v)
+  }}}
+    txn_Load #l (#blk, #off, #1)
+  {{{ (buf : Slice.t) b, RET (slice_val buf);
+      is_slice buf u8T [b] ∗
+      ⌜b = #0 <-> v = false⌝
+  }}}.
+Proof.
+Admitted.
+
+Theorem wp_txn_Load_inode l gBits gInodes gBlocks (blk off : u64)
+    (hG : gen_heapG u64 (updatable_buf inode_buf) Σ) v :
+  {{{ is_txn l gBits gInodes gBlocks ∗
+      ⌜gInodes !! blk = Some hG⌝ ∗
+      mapsto (hG := hG) off 1 (Stable v)
+  }}}
+    txn_Load #l (#blk, #off, #(inode_bytes*8))
+  {{{ (buf : Slice.t) vals, RET (slice_val buf);
+      is_slice buf u8T vals ∗
+      ⌜vals = inode_to_vals v⌝ }}}.
+Proof.
+Admitted.
+
+Theorem wp_txn_Load_block l gBits gInodes gBlocks (blk off : u64)
+    (hG : gen_heapG u64 (updatable_buf Block) Σ) v :
+  {{{ is_txn l gBits gInodes gBlocks ∗
+      ⌜gBlocks !! blk = Some hG⌝ ∗
+      mapsto (hG := hG) off 1 (Stable v)
+  }}}
+    txn_Load #l (#blk, #off, #(block_bytes*8))
+  {{{ (buf : Slice.t) vals, RET (slice_val buf);
+      is_slice buf u8T vals ∗
+      ⌜vals = Block_to_vals v⌝ }}}.
+Proof.
+Admitted.
+
+Axiom txn_CommitWait : val.
+
+Definition commit_pre
+    (gBits   : gmap u64 (gen_heapG u64 (updatable_buf bool) Σ))
+    (gInodes : gmap u64 (gen_heapG u64 (updatable_buf inode_buf) Σ))
+    (gBlocks : gmap u64 (gen_heapG u64 (updatable_buf Block) Σ))
+    (b : val) : iProp Σ :=
+  (
+    ∃ (bloc : loc) (blkno off sz : u64) data data_vals,
+      ⌜b = #bloc⌝ ∗
+      bloc ↦[struct.t buf.Buf.S] (#blkno, #off, #sz, slice_val data) ∗
+      is_slice data u8T data_vals ∗
+      (
+        ( ∃ (hG : gen_heapG u64 (updatable_buf bool) Σ) v,
+          ⌜sz=1⌝ ∗
+          ⌜gBits !! blkno = Some hG⌝ ∗
+          mapsto (hG := hG) off 1 (Stable v) ) ∨
+        ( ∃ (hG : gen_heapG u64 (updatable_buf inode_buf) Σ) v,
+          ⌜sz=inode_bits⌝ ∗
+          ⌜gInodes !! blkno = Some hG⌝ ∗
+          mapsto (hG := hG) off 1 (Stable v) ) ∨
+        ( ∃ (hG : gen_heapG u64 (updatable_buf Block) Σ) v,
+          ⌜sz=block_bits⌝ ∗
+          ⌜gBlocks !! blkno = Some hG⌝ ∗
+          mapsto (hG := hG) off 1 (Stable v) )
+      )
+  )%I.
+
+Definition commit_post
+    (gBits   : gmap u64 (gen_heapG u64 (updatable_buf bool) Σ))
+    (gInodes : gmap u64 (gen_heapG u64 (updatable_buf inode_buf) Σ))
+    (gBlocks : gmap u64 (gen_heapG u64 (updatable_buf Block) Σ))
+    (b : val) : iProp Σ :=
+  (
+    ∃ (bloc : loc) (blkno off sz : u64) data data_vals,
+      ⌜b = #bloc⌝ ∗
+      bloc ↦[struct.t buf.Buf.S] (#blkno, #off, #sz, slice_val data) ∗
+      is_slice data u8T data_vals ∗
+      (
+        ( ∃ (hG : gen_heapG u64 (updatable_buf bool) Σ) v,
+          ⌜sz=1⌝ ∗
+          ⌜gBits !! blkno = Some hG⌝ ∗
+          mapsto (hG := hG) off 1 (Stable v) ∗
+          ⌜ v = false ∧ data_vals = (#0 :: nil) ∨
+            v = true ∧ ∃ x, data_vals = [x] ∧ x ≠ #0 ⌝
+          ) ∨
+        ( ∃ (hG : gen_heapG u64 (updatable_buf inode_buf) Σ) v,
+          ⌜sz=inode_bits⌝ ∗
+          ⌜gInodes !! blkno = Some hG⌝ ∗
+          mapsto (hG := hG) off 1 (Stable v) ∗
+          ⌜ inode_to_vals v = data_vals ⌝ ) ∨
+        ( ∃ (hG : gen_heapG u64 (updatable_buf Block) Σ) v,
+          ⌜sz=block_bits⌝ ∗
+          ⌜gBlocks !! blkno = Some hG⌝ ∗
+          mapsto (hG := hG) off 1 (Stable v) ∗
+          ⌜ Block_to_vals v = data_vals ⌝ )
+      )
+  )%I.
+
+Theorem wp_txn_CommitWait l gBits gInodes gBlocks bufs buflist :
+  {{{ is_txn l gBits gInodes gBlocks ∗
+      is_slice bufs (refT (struct.t buf.Buf.S)) buflist ∗
+      ( [∗ list] _ ↦ buf ∈ buflist, commit_pre gBits gInodes gBlocks buf )
+  }}}
+    txn_CommitWait #l (slice_val bufs)
+  {{{ RET #();
+      is_slice bufs (refT (struct.t buf.Buf.S)) buflist ∗
+      ( [∗ list] _ ↦ buf ∈ buflist, commit_post gBits gInodes gBlocks buf ) }}}.
+Proof.
+Admitted.
 
 End heap.
